src/drf/PromiseIndep.v
@@ -1,0 +1,54 @@
+Require Import Omega.
+Require Import RelationClasses.
+
+Require Import sflib.
+
+Require Import Axioms.
+Require Import Basic.
+Require Import DataStructure.
+Require Import Time.
+Require Import Event.
+Require Import Language.
+Require Import Memory.
+Require Import Commit.
+Require Import Thread.
+Require Import Configuration.
+
+Set Implicit Arguments.
+
+
+Inductive pi_thread_step lang: forall (e:option Event.t) (readinfo:option (Loc.t * Time.t)) (e1 e2:Thread.t lang), Prop :=
+| pi_step_promise
+    e1 e2
+    (STEP: Thread.promise_step e1 e2):
+    pi_thread_step None None e1 e2
+| pi_step_program
+    e readinfo e1 e2
+    (STEP: Thread.program_step e readinfo e1 e2):
+    pi_thread_step e readinfo e1 e2
+.
+
+Inductive pi_step (tid:Ident.t) (e:option Event.t) (c1:Configuration.t): forall (c2:Configuration.t), Prop :=
+| pi_step_intro
+    readinfo lang st1 lc1 e2 st3 lc3 memory3
+    (TID: IdentMap.find tid c1.(Configuration.threads) = Some (existT _ lang st1, lc1))
+    (STEPS: rtc (Thread.step None) (Thread.mk _ st1 lc1 c1.(Configuration.memory)) e2)
+    (STEP: pi_thread_step e readinfo e2 (Thread.mk _ st3 lc3 memory3))
+    (READINFO: forall loc ts (READINFO: readinfo = Some (loc, ts)), ~ Threads.is_promised loc ts c1.(Configuration.threads)):
+    pi_step tid e c1 (Configuration.mk (IdentMap.add tid (existT _ _ st3, lc3) c1.(Configuration.threads)) memory3)
+.
+
+Inductive pi_step_except (tid_except:Ident.t) (c1 c2:Configuration.t): Prop :=
+| pi_step_neq_intro
+    tid e
+    (PI_STEP: pi_step tid e c1 c2)
+    (TID: tid <> tid_except)
+.
+
+Definition pi_consistent (c1:Configuration.t): Prop :=
+  forall tid c2
+    (TID: IdentMap.find tid c1.(Configuration.threads) <> None)
+    (STEPS: rtc (pi_step_except tid) c1 c2),
+  exists c3 lang st3 lc3,
+    <<STEPS: rtc (pi_step tid None) c2 c3>> /\
+    <<PROMISES: IdentMap.find tid c1.(Configuration.threads) = Some (existT _ lang st3, lc3)>>.
