src/lang/Progress.v
@@ -19,8 +19,8 @@ Set Implicit Arguments.
 
 Lemma program_step_promise
       lang
-      e st1 lc1 mem1 st2 lc2 mem2
-      (STEP: Thread.program_step e (Thread.mk lang st1 lc1 mem1) (Thread.mk lang st2 lc2 mem2))
+      e readinfo st1 lc1 mem1 st2 lc2 mem2
+      (STEP: Thread.program_step e readinfo (Thread.mk lang st1 lc1 mem1) (Thread.mk lang st2 lc2 mem2))
       (PROMISES: lc1.(Local.promises) = Memory.bot):
   lc2.(Local.promises) = Memory.bot.
 Proof.
